src/TotalMap.v
@@ -3,358 +3,11 @@ Local Set Warnings "-notation-overridden".
 From mathcomp Require Import ssreflect.ssrnat eqtype seq.
 From Coq Require Export Arith.Arith Bool.Bool.
 From Coq Require Import Logic.FunctionalExtensionality.
-From PolyAI Require Export ssrstring.
+From PolyAI Require Import Tactic.
 
 (* This code is inspired from the programming language fundations book *)
 
-Local Open Scope string_scope.
 Local Open Scope list_scope.
-
-
-(*  _____     _        _ __  __              *)
-(* |_   _|__ | |_ __ _| |  \/  | __ _ _ __   *)
-(*   | |/ _ \| __/ _` | | |\/| |/ _` | '_ \  *)
-(*   | | (_) | || (_| | | |  | | (_| | |_) | *)
-(*   |_|\___/ \__\__,_|_|_|  |_|\__,_| .__/  *)
-(*                                   |_|     *)
-
-
-(* Representation of a total map with finite non-default values *)
-
-Inductive total_map {Key: eqType} {Value} :=
-| TEmpty (v: Value)
-| TUpdate (m: total_map) (k: Key) (v: Value)
-.
-
-(* Notation for a default map *)
-Notation "'_' '!->' v" := (TEmpty v)
-  (at level 100, right associativity).
-
-(* Notation for a map update *)
-Notation "k '!->' v ';' m" := (TUpdate m k v)
-                                (at level 100, v at next level, right associativity).
-
-Fixpoint eqmap {Key: eqType} {Value: eqType} (m1 m2: @total_map Key Value) :=
-  match (m1, m2) with
-  | (TEmpty v1, TEmpty v2) => v1 == v2
-  | (TUpdate m1' k1 v1, TUpdate m2' k2 v2) => (eqmap m1' m2') && (k1 == k2) && (v1 == v2)
-  | _ => false
-  end.
-
-Theorem eqmapP {Key: eqType} {Value: eqType} :
-  Equality.axiom (@eqmap Key Value).
-Proof.
-  elim => [ v1 m2 /= | m1' Hind1 k1 v1 m2 /= ].
-  - apply (iffP idP).
-    + by case m2 => [ v2 /eqP -> // | // ].
-    + case m2 => [ v2 Heq | // ].
-        by injection Heq => ->.
-  - apply (iffP idP) => [ | <- ].
-    + by case m2 => [ // | m2' k2 v2 /andP[/andP[/Hind1 -> /eqP ->] /eqP ->]].
-    + rewrite !eq_refl.
-        by have -> : (eqmap m1' m1') by apply /Hind1.
-Qed.
-
-Canonical total_map_eqMixin {Key Value: eqType} := EqMixin (@eqmapP Key Value).
-Canonical total_map_eqType {Key Value: eqType} := Eval hnf in EqType (@total_map Key Value) total_map_eqMixin.
-
-(* Evaluate a map on a point*)
-Fixpoint eval_map {Key: eqType} {Value: Type} (m: @total_map Key Value) (k: Key) :=
-  match m with
-  | TEmpty v => v
-  | TUpdate m' k' v => if k' == k then v else eval_map m' k
-  end.
-
-(* Coercion for evaluation *)
-Coercion eval_map : total_map >-> Funclass.
-
-(* Useful lemmas and theorems *)
-
-Lemma t_apply_empty {Key: eqType} {Value: Type} (k: Key) (v: Value) :
-    (_ !-> v) k = v.
-Proof.
-  by [].
-Qed.
-
-Lemma t_update_eq {Key : eqType} {Value: Type} (m : total_map) (k: Key) (v: Value) :
-    (k !-> v ; m) k = v.
-Proof.
-  by rewrite /= eq_refl.
-Qed.
-
-Theorem t_update_neq {Key: eqType} {Value : Type} (m : total_map) (k1 k2: Key) (v: Value) :
-    k1 != k2 ->
-    (k1 !-> v ; m) k2 = m k2.
-Proof.
-  by move => /negb_true_iff /= ->.
-Qed.
-
-Lemma t_update_shadow {Key: eqType} {Value: Type} (m : total_map) (k: Key) (v1 v2: Value) :
-    eval_map (k !-> v2 ; k !-> v1 ; m) = eval_map (k !-> v2 ; m).
-Proof.
-  extensionality k' => /=.
-  by case (k == k').
-Qed.
-
-Theorem t_update_same {Key : eqType} {Value: Type} (m : @total_map Key Value) (k: Key) :
-    eval_map (k !-> m k ; m) = eval_map m.
-Proof.
-  extensionality k' => /=.
-  by case (k =P k') => [-> | ].
-Qed.
-
-Theorem t_update_permute {Key : eqType} {Value: Type} (m : total_map) (k1 k2: Key) (v1 v2: Value) :
-    k2 != k1 ->
-    eval_map (k1 !-> v1 ; k2 !-> v2 ; m) =
-    eval_map (k2 !-> v2 ; k1 !-> v1 ; m).
-Proof.
-  move => /negb_true_iff Hne /=.
-  extensionality k'.
-  case (k1 =P k') => [ <- /= | _ //].
-  - by rewrite Hne.
-Qed.
-
-Require Import Coq.ZArith.BinInt.
-
-(* Pointwise operations on one or multiple maps *)
-
-Fixpoint pointwise_un_op {Key: eqType} {Value Value': Type} (m: @total_map Key Value) (f: Value -> Value') :=
-  match m with
-  | TEmpty v => (_ !-> f v)
-  | TUpdate m1' k v => let new_m := pointwise_un_op m1' f in
-                      (k !-> f v; new_m)
-  end.
-
-Theorem pointwise_un_op_spec {Key: eqType} {Value Value': Type} (m: @total_map Key Value) (f: Value -> Value') (k: Key) :
-  (pointwise_un_op m f) k = f (m k).
-Proof.
-  elim: m f k => [// | m Hind k v f k' /=].
-  rewrite Hind.
-  by case (k == k').
-Qed.
-
-Fixpoint pointwise_un_op_in_seq {Key: eqType} {Value: Type} (m: @total_map Key Value) (f: Value -> Value) (l: seq Key) :=
-  match l with
-  | [::] => m
-  | a::l' => (a !-> f (m a); pointwise_un_op_in_seq m f l')
-  end.
-
-Theorem pointwise_un_op_in_seq_spec {Key: eqType} {Value: Type} (m: @total_map Key Value) (f: Value -> Value) (l: seq Key) :
-  forall x, (pointwise_un_op_in_seq m f l) x = if x \in l then f (m x) else (m x).
-Proof.
-  move => x. elim: l => [// | k l'].
-  rewrite in_cons. case: (x \in l') => Hind /=; case: (x =P k) => [-> | /eqP /negb_true_iff].
-  - by rewrite eq_refl.
-  - by rewrite eq_sym => ->.
-  - by rewrite eq_refl.
-  - by rewrite eq_sym => ->.
-Qed.
-
-Fixpoint pointwise_bin_op_aux {Key: eqType} {Value1 Value2 Value3: Type} (m1: @total_map Key Value1)
-         (k2: Value2) (f: Value1 -> Value2 -> Value3) :=
-  match m1 with
-  | TEmpty k1 => (_ !-> f k1 k2)
-  | TUpdate m1' v k1 => let new_m := pointwise_bin_op_aux m1' k2 f in
-                       (v !-> f k1 k2; new_m)
-  end.
-
-Lemma pointwise_bin_op_aux_spec {Key: eqType} {Value1 Value2 Value3: Type} (m1: @total_map Key Value1)
-      (v2: Value2) (f: Value1 -> Value2 -> Value3) (k: Key):
-  (pointwise_bin_op_aux m1 v2 f) k = f (m1 k) v2.
-Proof.
-  elim: m1 => [// | m1 Hind k1 v1 /=].
-  rewrite Hind.
-  by case (k1 == k).
-Qed.
-
-Fixpoint pointwise_bin_op {Key: eqType} {Value1 Value2 Value3: Type} (m1: @total_map Key Value1)
-         (m2: @total_map Key Value2) (f: Value1 -> Value2 -> Value3) :=
-  match m2 with
-  | TEmpty v2 => pointwise_bin_op_aux m1 v2 f
-  | TUpdate m2' k v2 => let new_m := pointwise_bin_op m1 m2' f in
-                       (k !-> (f (m1 k) v2); new_m)
-  end.
-
-Theorem pointwise_bin_op_spec {Key: eqType} {Value1 Value2 Value3: Type} (m1: @total_map Key Value1)
-         (m2: @total_map Key Value2) (f: Value1 -> Value2 -> Value3) (k: Key):
-  (pointwise_bin_op m1 m2 f) k = f (m1 k) (m2 k).
-Proof.
-  elim: m2 m1 => [v m1 | m2 Hind k2 v2 m1 /=].
-  - by apply pointwise_bin_op_aux_spec.
-  - rewrite Hind.
-    by case (k2 =P k) => [-> // | //].
-Qed.
-
-Local Open Scope string_scope.
-
-Lemma ne_length_impl_ne :
-  forall s1 s2, length s1 <> length s2 -> s1 <> s2.
-Proof.
-  move => s1 s2 HLength Heq.
-  rewrite Heq in HLength.
-    by case HLength.
-Qed.
-
-Lemma string_append_length :
-  forall s1 s2, length (s1 ++ s2) = length s1 + length s2.
-Proof.
-  elim => [s2 // | a s1 Hind s2 /=].
-    by rewrite Hind.
-Qed.
-
-Fixpoint repeat_string (n: nat) :=
-  match n with
-  | O => ""
-  | S n' => "X" ++ (repeat_string n')
-  end.
-
-Lemma repeat_string_length :
-  forall n, length (repeat_string n) = n.
-Proof.
-  elim => [// | n Hind /=].
-  by auto.
-Qed.
-
-Fixpoint construct_not_in_list (l: list string) :=
-  match l with
-  | nil => "X"
-  | a::l' => (repeat_string (length a)) ++ (construct_not_in_list l')
-  end.
-
-Lemma construct_not_in_list_length :
-  forall l, 0 < length (construct_not_in_list l).
-Proof.
-  elim => [// | a l Hind /=].
-  rewrite string_append_length.
-    by apply ltn_addl.
-Qed.
-
-Theorem construct_not_in_list_length_forall :
-  forall l x, x \in l -> length (construct_not_in_list l) > length x.
-Proof.
-  elim => [x Hin /= // | a l Hind x /=].
-  rewrite in_cons => /orP [/eqP -> | Hinl].
-  - rewrite string_append_length repeat_string_length.
-    rewrite {1}(plus_n_O (length a)).
-    by rewrite ltn_add2l construct_not_in_list_length.
-  - rewrite string_append_length ltn_addl => //.
-    by auto.
-Qed.
-
-Theorem construct_not_in_list_spec:
-  forall l, (construct_not_in_list l) \notin l.
-Proof.
-  move => l. apply /negP => HIn.
-  apply construct_not_in_list_length_forall in HIn.
-    by rewrite ltnn in HIn.
-Qed.
-
-Fixpoint forall_bin_op_aux {Value: Type} (m1: total_map) (v2: Value)
-         (f: Value -> Value -> bool) (seen: list string) :=
-  match m1 with
-  | TEmpty v1 => f v1 v2
-  | TUpdate m1' k v1 =>
-    if k \in seen then
-      forall_bin_op_aux m1' v2 f seen
-    else
-      f v1 v2 && forall_bin_op_aux m1' v2 f (k::seen)
-  end.
-
-Lemma forall_bin_op_aux_spec {Value: Type} {m1: total_map} (v2: Value)
-      (f: Value -> Value -> bool) (seen: list string) :
-  forall_bin_op_aux m1 v2 f seen <->
-                       (forall k, k \notin seen -> f (m1 k) v2).
-Proof.
-  elim: m1 seen => [v seen /= | m Hind k v1 seen /=].
-    by split => [// | H]; apply (H (construct_not_in_list seen)), construct_not_in_list_spec.
-    case_eq (k \in seen) => Hseen.
-  - rewrite Hseen Hind.
-    split => [Hin k0 HnotIn | Hin k0 /negP Hf]; move: Hseen.
-    + case (k =P k0) => [-> Hin2 | //]; auto.
-      move => /negb_true_iff in HnotIn. by rewrite Hin2 in HnotIn.
-    + case (k =P k0) => [-> // | /eqP /negb_true_iff Hkk0].
-      move => /negP in Hf. apply Hin in Hf.
-        by rewrite Hkk0 in Hf.
-  - rewrite Hseen. split => [/andP[Hf /Hind Hforall] k0 Hk0notin | H ].
-    + case (k =P k0) => [// | Hkk0 ].
-      apply Hforall. rewrite in_cons. apply /norP. split; auto.
-      apply /eqP. auto.
-    + move => /negb_true_iff in Hseen.
-      apply /andP. split.
-      * apply H in Hseen.
-          by rewrite eq_refl in Hseen.
-      * apply Hind => k0 /=. rewrite in_cons => /norP [/negb_true_iff Hkk0 /H Hnotin].
-          by rewrite eq_sym Hkk0 in Hnotin.
-Qed.
-
-Fixpoint forall_bin_op_fix {Value: Type} (m1 m2: total_map) (f: Value -> Value -> bool) (seen: list string):=
-  match m2 with
-  | TEmpty v2 => forall_bin_op_aux m1 v2 f seen
-  | TUpdate m2' k v2 =>
-    if k \in seen then
-      forall_bin_op_fix m1 m2' f seen
-    else
-      f (m1 k) v2 && forall_bin_op_fix m1 m2' f (k::seen)
-  end.
-
-Lemma forall_bin_op_fix_spec {Value: Type} (m1 m2: total_map) (f: Value -> Value -> bool) (seen: list string) :
-  forall_bin_op_fix m1 m2 f seen <-> forall k, k \notin seen -> f (m1 k) (m2 k).
-Proof.
-  elim: m2 m1 seen => [v1 m2 seen /= | m2 Hind k v1 m1 seen /=].
-    by split => /forall_bin_op_aux_spec.
-  case_eq (k \in seen) => Hseen. rewrite Hseen.
-  - rewrite Hind.
-    split => [Hin k0 HnotIn| HIn k0 Hf]; move: Hseen.
-    + case (k =P k0) => [-> | //]; auto.
-      move => /negb_true_iff in HnotIn. by rewrite HnotIn.
-    + case (k =P k0) => [-> // | Hkk0].
-      * move => /negb_true_iff in Hf. by rewrite Hf.
-      * move: Hf => /HIn.
-          by move: Hkk0 => /eqP /negb_true_iff ->.
-  - rewrite Hseen. split => [/andP[Hf /Hind Hforall] k0 Hk0notin | H ].
-    + case (k =P k0) => [<- // | Hkk0].
-      apply Hforall. rewrite in_cons. apply /norP. split; auto. apply /eqP. auto.
-    + apply /andP. split.
-      * move => /negb_true_iff in Hseen. apply H in Hseen.
-          by rewrite eq_refl in Hseen.
-      * apply Hind => v0 /=. rewrite in_cons => /norP [/negb_true_iff Hvv0 /H Hnotin].
-          by rewrite eq_sym Hvv0 in Hnotin.
-Qed.
-
-Definition forall_bin_op {Value: Type} (m1 m2: total_map) (f: Value -> Value -> bool) :=
-  forall_bin_op_fix m1 m2 f nil.
-
-Theorem forall_bin_op_spec {Value: Type} (m1 m2: total_map) (f: Value -> Value -> bool) :
-  forall_bin_op m1 m2 f <-> forall k, f (m1 k) (m2 k).
-Proof.
-  rewrite forall_bin_op_fix_spec /=.
-  split; auto.
-Qed.
-
-(* Useful tactic which apply known lemmas *)
-
-Ltac simpl_totalmap :=
-repeat match goal with
-       | [ |- context[eval_map (_ !-> _) _] ] => rewrite t_apply_empty
-       | [ |- context[eval_map (?k !-> _ ; _) ?k]] => rewrite t_update_eq
-       | [ H : ?k1 <> ?k2 |- _ ] => move: H => /eqP H
-
-       | [ H : is_true (?k1 != ?k2) |- context[eval_map (?k1 !-> _ ; _) ?k2] ] => rewrite (t_update_neq _ _ _ _ H)
-       | [ H : is_true (?k2 != ?k1) |- context[eval_map (?k1 !-> _ ; _) ?k2] ] =>
-         rewrite eq_sym in H; rewrite (t_update_neq _ _ _ _ H); rewrite eq_sym in H
-       | [ |- context[eval_map (?k1 !-> _ ; ?m) ?k2]] => rewrite (t_update_neq m k1 k2 _); last first; [ by [] | idtac ]
-       | [ |- context[eval_map (?k !-> _ ; ?k !-> _ ; _)]] => rewrite t_update_shadow
-       | [ |- context[eval_map (?k !-> eval_map ?m ?k ; ?m)]] => rewrite t_update_same
-       | [ |- context[(?k == ?k)]] => rewrite eq_refl
-       | [ |- context[eval_map (pointwise_un_op _ _) _]] => rewrite pointwise_un_op_spec
-       | [ |- context[eval_map (pointwise_bin_op _ _ _) _]] => rewrite pointwise_bin_op_spec
-       | [ |- is_true (forall_bin_op _ _ _)] => apply forall_bin_op_spec
-       | [ H : is_true ?x |- context[?x]] => rewrite H
-       | [ H : is_true (?x != ?y) |- context[?x == ?y]] => rewrite ?(ifN_eq _ _ H) ?(ifN_eqC _ _ H)
-       | _ => rewrite //=; auto
-       end.
-
-Global Opaque eval_map.
 
 (*  ____            _   _       _ __  __              *)
 (* |  _ \ __ _ _ __| |_(_) __ _| |  \/  | __ _ _ __   *)
@@ -519,3 +172,179 @@ repeat match goal with
        end.
 
 Global Opaque eval_partial_map.
+
+(*  _____     _        _ __  __            ____   *)
+(* |_   _|__ | |_ __ _| |  \/  | __ _ _ __|___ \  *)
+(*   | |/ _ \| __/ _` | | |\/| |/ _` | '_ \ __) | *)
+(*   | | (_) | || (_| | | |  | | (_| | |_) / __/  *)
+(*   |_|\___/ \__\__,_|_|_|  |_|\__,_| .__/_____| *)
+(*                                   |_|          *)
+
+(* Representation of a total map with finite non-default values *)
+
+Section TotalMapDefinition.
+
+  Context (Key: eqType) (Value: Type).
+
+  Structure total_map := TotalMap
+    {
+      t_map: @partial_map Key Value;
+      t_default: Value;
+    }.
+
+End TotalMapDefinition.
+
+Section TotalMapCoreDefinitions.
+
+  Context {Key: eqType} {Value: Type}.
+
+  (* Update the total map *)
+  Definition t_update (m: total_map Key Value) (k: Key) (v: Value) :=
+    TotalMap _ _ (k !!-> v; t_map _ _ m) (t_default _ _ m).
+
+End TotalMapCoreDefinitions.
+
+(* Notation for a map update *)
+Notation "k '!->' v ';' m" := (t_update m k v)
+                                 (at level 100, v at next level, right associativity).
+
+(* Notation for a default map *)
+Notation "'_' '!->' v" := (TotalMap _ _ (PEmpty) v)
+                             (at level 100).
+
+
+Section TotalMapEqType.
+
+  Context {Key Value: eqType}.
+
+  Definition eq_total_map (m1 m2: total_map Key Value) :=
+    ((t_map _ _ m1) == t_map _ _ m2) && (t_default _ _ m1 == t_default _ _ m2).
+
+  Theorem eq_total_mapP :
+    Equality.axiom (eq_total_map).
+  Proof.
+    move => [map1 default1] [map default2].
+    apply (iffP idP) => [ /andP /= [/eqP -> /eqP ->] // | -> ].
+    rewrite /eq_total_map. by rewrite !eq_refl.
+  Qed.
+
+  Canonical total_map_eqMixin := EqMixin (eq_total_mapP).
+  Canonical total_map_eqType := Eval hnf in EqType (@total_map Key Value) total_map_eqMixin.
+
+End TotalMapEqType.
+
+Section TotalMapEval.
+
+  (* Evaluate a map on a point*)
+  Definition eval_total_map {Key: eqType} {Value: Type} (m: @total_map Key Value) (k: Key) :=
+    if (t_map _ _ m) k is Some v then
+      v
+    else
+      t_default _ _ m.
+
+  (* Coercion for evaluation *)
+  Coercion eval_total_map : total_map >-> Funclass.
+
+End TotalMapEval.
+
+(* Important rewrite rules *)
+Section TotalMapRewriteRules.
+
+  Context {Key: eqType} {Value: Type} (k k1 k2: Key) (v v1 v2: Value) (m: total_map Key Value).
+
+  Lemma t_update_out (pm: partial_map):
+    eval_total_map (TotalMap _ _ (k !!-> v1 ; pm) v) = eval_total_map (t_update (TotalMap _ _ pm v) k v1).
+  Proof.
+      by [].
+  Qed.
+
+  Lemma t_apply_empty :
+    (_ !-> v) k = v.
+  Proof.
+      by [].
+  Qed.
+
+  Lemma t_update_eq :
+    (k !-> v ; m) k = v.
+  Proof.
+    rewrite /eval_total_map.
+      by simpl_partialmap.
+  Qed.
+
+  Theorem t_update_neq :
+    k1 != k2 ->
+    (k1 !-> v ; m) k2 = m k2.
+  Proof.
+    move => Hne. rewrite /eval_total_map.
+      by simpl_partialmap.
+  Qed.
+
+  Lemma t_update_shadow :
+    eval_total_map (k !-> v2 ; k !-> v1 ; m) = eval_total_map (k !-> v2 ; m).
+  Proof.
+    rewrite /eval_total_map.
+    extensionality k' => /=.
+      by simpl_partialmap.
+  Qed.
+
+  Theorem t_update_same :
+    eval_total_map (k !-> m k ; m) = eval_total_map m.
+  Proof.
+    rewrite /eval_total_map.
+    extensionality k' => /=.
+    case (k =P k') => [ -> | /eqP Hne ]; by simpl_partialmap.
+  Qed.
+
+  Theorem t_update_permute :
+    k2 != k1 ->
+    eval_total_map (k1 !-> v1 ; k2 !-> v2 ; m) =
+    eval_total_map (k2 !-> v2 ; k1 !-> v1 ; m).
+  Proof.
+    rewrite /eval_total_map => Hne.
+    extensionality k' => /=.
+      by rewrite p_update_permute.
+  Qed.
+
+End TotalMapRewriteRules.
+
+Hint Rewrite @t_update_out @t_apply_empty @t_update_eq @t_update_neq @t_update_shadow @t_update_same using by simplssr : totalrw.
+
+(* Pointwise operations on one or multiple maps *)
+
+Section TotalMapPointwiseUn.
+
+  Context {Key: eqType}
+          {Value Value': Type}.
+
+  Definition t_pointwise_un_op (m: total_map Key Value) (f: Value -> Value') :=
+    TotalMap _ _ (p_pointwise_un_op (t_map _ _ m) f) (f (t_default _ _ m)).
+
+  Theorem t_pointwise_un_op_spec (m: total_map Key Value) (f: Value -> Value') (k: Key) :
+    t_pointwise_un_op m f k = f (m k).
+  Proof.
+    rewrite /t_pointwise_un_op /eval_total_map /=.
+    simpl_partialmap.
+    by case (t_map _ _ m k).
+  Qed.
+
+  Fixpoint t_pointwise_un_op_in_seq (m: total_map Key Value) (f: Value -> Value) (l: seq Key) :=
+    match l with
+    | [::] => m
+    | a::l' => (a !-> f (m a); t_pointwise_un_op_in_seq m f l')
+    end.
+
+  Theorem t_pointwise_un_op_in_seq_spec (m: total_map Key Value) (f: Value -> Value) (l: seq Key) :
+    forall x, (t_pointwise_un_op_in_seq m f l) x = if x \in l then f (m x) else (m x).
+  Proof.
+    move => x. elim l => [ // | k l' ].
+    rewrite in_cons. case: (x \in l') => Hind /=; case: (x =P k) => [ -> | /eqP Hne ]; by autorewrite with totalrw.
+  Qed.
+
+End TotalMapPointwiseUn.
+
+Hint Rewrite @t_pointwise_un_op_spec @t_pointwise_un_op_in_seq_spec using by reflect_ne ; simplssr : totalrw.
+
+Global Opaque eval_total_map.
+
+Ltac simpl_totalmap_ := repeat simplssr ; autorewrite with totalrw; simplssr.
+Ltac simpl_totalmap := reflect_ne_in simpl_totalmap_.
