src/Tactic.v
@@ -1,0 +1,31 @@
+From Coq Require Import ssreflect ssrfun ssrbool.
+From mathcomp Require Import eqtype.
+
+Ltac rewrite_is_true :=
+  repeat match goal with
+         | [ H: is_true ?e |- context[?e] ] => rewrite H
+         | [ H: is_true (negb ?e) |- context[?e] ] => move => /negb_true_iff in H; rewrite H; move => /negb_true_iff in H
+         | _ => rewrite /=
+         end.
+
+Ltac simpleq :=
+  repeat match goal with
+         | [ H: is_true (?x != ?y) |- context[?y == ?x] ] => rewrite eq_sym in H; rewrite_is_true; rewrite eq_sym in H
+         | [ H: is_true (?x == ?y) |- context[?y == ?x] ] => rewrite eq_sym in H; rewrite_is_true; rewrite eq_sym in H
+         | [ |- context[?x == ?x] ] => rewrite (eq_refl _ ?x)
+         | _ => rewrite /=
+         end.
+
+Ltac reflect_ne_in tac :=
+  repeat match goal with
+         | [ H: ?x <> ?y |- _ ] => move => /eqP in H
+         | _ => tac
+         end.
+
+Ltac reflect_ne :=
+  repeat match goal with
+         | [ H: ?x <> ?y |- _ ] => move => /eqP in H
+         | _ => idtac
+         end.
+
+Ltac simplssr := rewrite_is_true; simpleq.
